SP1Operations/Compare/IsEqualWordOperation/Constraints.lean
@@ -5,19 +5,19 @@ namespace IsEqualWordOperation
 
 section constraints
 
-@[irreducible] def constraints
-  (a : (Word (Fin KB)))
-  (b : (Word (Fin KB)))
-  (cols : IsEqualWordOperation)
-  (is_real : (Fin KB))
-  : SP1ConstraintList (Fin KB) :=
-  let E0 : Fin KB := is_real - 1
-  let E1 : Fin KB := is_real * E0
-  let E2 : Fin KB := a[0] - b[0]
-  let E3 : Fin KB := a[1] - b[1]
-  let E4 : Fin KB := a[2] - b[2]
-  let E5 : Fin KB := a[3] - b[3]
-  let CS0 : SP1ConstraintList (Fin KB) := IsZeroWordOperation.constraints #v[E2, E3, E4, E5] { is_zero_limb := #v[{ inverse := cols.is_diff_zero.is_zero_limb[0].inverse, result := cols.is_diff_zero.is_zero_limb[0].result }, { inverse := cols.is_diff_zero.is_zero_limb[1].inverse, result := cols.is_diff_zero.is_zero_limb[1].result }, { inverse := cols.is_diff_zero.is_zero_limb[2].inverse, result := cols.is_diff_zero.is_zero_limb[2].result }, { inverse := cols.is_diff_zero.is_zero_limb[3].inverse, result := cols.is_diff_zero.is_zero_limb[3].result }], is_zero_first_half := cols.is_diff_zero.is_zero_first_half, is_zero_second_half := cols.is_diff_zero.is_zero_second_half, result := cols.is_diff_zero.result } is_real
+@[irreducible] def constraints {F : Type} [Field F]
+  (a : (Word F))
+  (b : (Word F))
+  (cols : IsEqualWordOperation F)
+  (is_real : F)
+  : SP1ConstraintList F :=
+  let E0 : F := is_real - 1
+  let E1 : F := is_real * E0
+  let E2 : F := a[0] - b[0]
+  let E3 : F := a[1] - b[1]
+  let E4 : F := a[2] - b[2]
+  let E5 : F := a[3] - b[3]
+  let CS0 : SP1ConstraintList F := IsZeroWordOperation.constraints #v[E2, E3, E4, E5] { is_zero_limb := #v[{ inverse := cols.is_diff_zero.is_zero_limb[0].inverse, result := cols.is_diff_zero.is_zero_limb[0].result }, { inverse := cols.is_diff_zero.is_zero_limb[1].inverse, result := cols.is_diff_zero.is_zero_limb[1].result }, { inverse := cols.is_diff_zero.is_zero_limb[2].inverse, result := cols.is_diff_zero.is_zero_limb[2].result }, { inverse := cols.is_diff_zero.is_zero_limb[3].inverse, result := cols.is_diff_zero.is_zero_limb[3].result }], is_zero_first_half := cols.is_diff_zero.is_zero_first_half, is_zero_second_half := cols.is_diff_zero.is_zero_second_half, result := cols.is_diff_zero.result } is_real
   CS0 ++ [
     (.assertZero E1),
   ]
