SP1Operations/Compare/IsEqualWordOperation/Operation.lean
@@ -1,4 +1,4 @@
 import SP1Operations.Compare.IsZeroWordOperation
 
-structure IsEqualWordOperation where
-  is_diff_zero : IsZeroWordOperation
+structure IsEqualWordOperation (F : Type) where
+  is_diff_zero : IsZeroWordOperation F
