SP1Operations/Compare/IsZeroWordOperation/Constraints.lean
@@ -5,26 +5,26 @@ namespace IsZeroWordOperation
 
 section constraints
 
-@[irreducible] def constraints
-  (a : (Word (Fin KB)))
-  (cols : IsZeroWordOperation)
-  (is_real : (Fin KB))
-  : SP1ConstraintList (Fin KB) :=
-  let CS0 : SP1ConstraintList (Fin KB) := IsZeroOperation.constraints a[0] { inverse := cols.is_zero_limb[0].inverse, result := cols.is_zero_limb[0].result } is_real
-  let CS1 : SP1ConstraintList (Fin KB) := IsZeroOperation.constraints a[1] { inverse := cols.is_zero_limb[1].inverse, result := cols.is_zero_limb[1].result } is_real
-  let CS2 : SP1ConstraintList (Fin KB) := IsZeroOperation.constraints a[2] { inverse := cols.is_zero_limb[2].inverse, result := cols.is_zero_limb[2].result } is_real
-  let CS3 : SP1ConstraintList (Fin KB) := IsZeroOperation.constraints a[3] { inverse := cols.is_zero_limb[3].inverse, result := cols.is_zero_limb[3].result } is_real
-  let E0 : Fin KB := is_real - 1
-  let E1 : Fin KB := is_real * E0
-  let E2 : Fin KB := cols.result - 1
-  let E3 : Fin KB := cols.result * E2
-  let E4 : Fin KB := cols.is_zero_limb[0].result * cols.is_zero_limb[1].result
-  let E5 : Fin KB := cols.is_zero_first_half - E4
-  let E6 : Fin KB := cols.is_zero_limb[2].result * cols.is_zero_limb[3].result
-  let E7 : Fin KB := cols.is_zero_second_half - E6
-  let E8 : Fin KB := cols.is_zero_first_half * cols.is_zero_second_half
-  let E9 : Fin KB := cols.result - E8
-  let E10 : Fin KB := is_real * E9
+@[irreducible] def constraints {F : Type} [Field F]
+  (a : (Word F))
+  (cols : IsZeroWordOperation F)
+  (is_real : F)
+  : SP1ConstraintList F :=
+  let CS0 : SP1ConstraintList F := IsZeroOperation.constraints a[0] { inverse := cols.is_zero_limb[0].inverse, result := cols.is_zero_limb[0].result } is_real
+  let CS1 : SP1ConstraintList F := IsZeroOperation.constraints a[1] { inverse := cols.is_zero_limb[1].inverse, result := cols.is_zero_limb[1].result } is_real
+  let CS2 : SP1ConstraintList F := IsZeroOperation.constraints a[2] { inverse := cols.is_zero_limb[2].inverse, result := cols.is_zero_limb[2].result } is_real
+  let CS3 : SP1ConstraintList F := IsZeroOperation.constraints a[3] { inverse := cols.is_zero_limb[3].inverse, result := cols.is_zero_limb[3].result } is_real
+  let E0 : F := is_real - 1
+  let E1 : F := is_real * E0
+  let E2 : F := cols.result - 1
+  let E3 : F := cols.result * E2
+  let E4 : F := cols.is_zero_limb[0].result * cols.is_zero_limb[1].result
+  let E5 : F := cols.is_zero_first_half - E4
+  let E6 : F := cols.is_zero_limb[2].result * cols.is_zero_limb[3].result
+  let E7 : F := cols.is_zero_second_half - E6
+  let E8 : F := cols.is_zero_first_half * cols.is_zero_second_half
+  let E9 : F := cols.result - E8
+  let E10 : F := is_real * E9
   CS0 ++ CS1 ++ CS2 ++ CS3 ++ [
     (.assertZero E1),
     (.assertZero E3),
