SP1Operations/Operation/U16MSBOperation/Operation.lean
@@ -1,4 +1,4 @@
 import SP1Foundations
 
-@[ext] structure U16MSBOperation where
-  msb : Fin KB
+@[ext] structure U16MSBOperation (F : Type*) where
+  msb : F
