SP1Operations/Compare/LtOperationSigned/Operation.lean
@@ -3,5 +3,5 @@ import SP1Operations.Compare.LtOperationUnsigned
 
 structure LtOperationSigned where
   result : LtOperationUnsigned
-  b_msb : U16MSBOperation
-  c_msb : U16MSBOperation
+  b_msb : U16MSBOperation (Fin KB)
+  c_msb : U16MSBOperation (Fin KB)
