SP1Operations/Compare/LtOperationUnsigned/Operation.lean
@@ -1,7 +1,7 @@
 import SP1Operations.Compare.U16CompareOperation
 
 structure LtOperationUnsigned where
-  u16_compare_operation : U16CompareOperation
+  u16_compare_operation : U16CompareOperation (Fin KB)
   u16_flags : Word (Fin KB)
   not_eq_inv : Fin KB
   comparison_limbs : Vector (Fin KB) 2
