SP1Operations/Compare/U16CompareOperation.lean
@@ -6,7 +6,7 @@ namespace U16CompareOperation
 @[grind →, aesop safe forward]
 lemma spec
   (a b : Fin KB)
-  (cols : U16CompareOperation)
+  (cols : U16CompareOperation (Fin KB))
   (h_a_isU16 : (a : ℕ) < 65536)
   (h_b_isU16 : (b : ℕ) < 65536) :
   List.Forall SP1Constraint.toProp (constraints a b cols 1) →
