SP1Operations/Operation/AddwOperation/Operation.lean
@@ -3,4 +3,4 @@ import SP1Operations.Operation.U16MSBOperation
 
 structure AddwOperation where
   value : Vector (Fin KB) 2
-  msb : U16MSBOperation
+  msb : U16MSBOperation (Fin KB)
